<?xml version="1.0" encoding="ISO-8859-1" standalone="yes"?>
<!--
  Data HUb Service (DHuS) - For Space data distribution.
  Copyright (C) 2013,2014,2015,2016 European Space Agency (ESA)
  Copyright (C) 2013,2014,2015,2016 GAEL Systems
  Copyright (C) 2013,2014,2015,2016 Serco Spa

  This file is part of DHuS software sources.

  This program is free software: you can redistribute it and/or modify
  it under the terms of the GNU Affero General Public License as
  published by the Free Software Foundation, either version 3 of the
  License, or (at your option) any later version.

  This program is distributed in the hope that it will be useful,
  but WITHOUT ANY WARRANTY; without even the implied warranty of
  MERCHANTABILITY or FITNESS FOR A PARTICULAR PURPOSE. See the
  GNU Affero General Public License for more details.

  You should have received a copy of the GNU Affero General Public License
  along with this program. If not, see <http://www.gnu.org/licenses/>.

-->


<!DOCTYPE rdf:RDF [
   <!ENTITY rdf  "http://www.w3.org/1999/02/22-rdf-syntax-ns#">
   <!ENTITY rdfs "http://www.w3.org/2000/01/rdf-schema#">
   <!ENTITY owl  "http://www.w3.org/2002/07/owl#">
   <!ENTITY s3   "http://www.esa.int/s3#">
   <!ENTITY drb  "http://www.gael.fr/drb#">
   <!ENTITY jpeg "http://www.gael.fr/drb/jpeg#">
]>
<rdf:RDF xmlns:owl="&owl;"
         xmlns:rdf="&rdf;"
         xmlns:rdfs="&rdfs;"
         xmlns:drb="&drb;"
         xmlns:jpeg="&jpeg;"
         xmlns:s3="&s3;"
         xml:base="&s3;">

   <owl:Ontology rdf:about="&s3;">
      <rdfs:label xml:lang="en">Sentinel-3 - Level-0 Ontology</rdfs:label>
   </owl:Ontology>


   <!-- =================================================================== -->
   <!--                                                                     -->
   <!-- IPF Level 0 Abstract class                                          -->
   <!--                                                                     -->
   <!-- =================================================================== -->
   
   <owl:Class rdf:about="&s3;ipf_level_0">
      <rdfs:label xml:lang="en">IPF Level-0</rdfs:label>
      <rdfs:comment xml:lang="en">
         IPF containing level-0 processing item. It consists on
         MSI raw-image-data (compressed) in raw ISP format.
      </rdfs:comment>      
      <rdfs:subClassOf rdf:resource="&s3;product"/>
      <drb:signature rdf:parseType="Resource">
         <drb:nameMatch>.*\_0_(SRA___|CAL___|MWR___|SLT___|EFR___|CR0___|CR1___|GNS___|NAV___|DOP___|HKM___|NAT___|HKM2__)_\d{8}T\d{6}_\d{8}T\d{6}_\d{8}T\d{6}_\w{17}_\w{3}_\w{8}.SEN3</drb:nameMatch>
      </drb:signature>
   </owl:Class>
   
   <owl:Class rdf:about="&s3;ipf_olci_level_0">
      <rdfs:label xml:lang="en">IPF Level-0 (OLCI) </rdfs:label>
      <rdfs:comment xml:lang="en">
         IPF containing level-0 processing item. It consists on
         MSI raw-image-data (compressed) in raw ISP format.
      </rdfs:comment>      
      <rdfs:subClassOf rdf:resource="&s3;ipf_level_0"/>
      <drb:signature rdf:parseType="Resource">
         <drb:nameMatch>S3[AB_]_OL_0_.*</drb:nameMatch>	  	 
      </drb:signature>
   </owl:Class>
   
   <owl:Class rdf:about="&s3;ipf_slstr_level_0">
      <rdfs:label xml:lang="en">IPF Level-0 (SLSTR) </rdfs:label>
      <rdfs:comment xml:lang="en">
         IPF containing level-0 processing item. It consists on
         many raw channels in ISP format (Optical, Fire, Scan, ancillary).
      </rdfs:comment>      
      <rdfs:subClassOf rdf:resource="&s3;ipf_level_0"/>
      <drb:signature rdf:parseType="Resource">
         <drb:nameMatch>S3[AB_]_SL_0_.*</drb:nameMatch>      
      </drb:signature>
   </owl:Class>
   

</rdf:RDF>
